src/lib/poly/Kuiper.Poly.AtomicReduce.fsti
@@ -5,8 +5,8 @@ module Kuiper.Poly.AtomicReduce
 #lang-pulse
 
 open Kuiper
+open Kuiper.Array1
 open Kuiper.Atomics
-
 
 noeq
 type is_ac_w (#t:Type) (f: t -> t -> t) = {
@@ -16,11 +16,13 @@ type is_ac_w (#t:Type) (f: t -> t -> t) = {
 
 inline_for_extraction noextract
 type reduce_ty
-  (et : Type0) {| scalar et |} {| d : has_atomic_add et |} =
+  (et : Type0) {| scalar et, d : has_atomic_add et |}
+  (r : (l:nat -> layout l))
+  =
   fn (ac : is_ac_w d.pure_op)
      (n : szp{n < max_blocks})
-     (a : gpu_array et n { is_global_array a })
-     (#v_a : erased (seq et))
+     (a : array1 et (r n) { is_global a })
+     (#v_a : erased (lseq et n))
   preserves cpu ** on gpu_loc (a |-> v_a)
   returns   r : et
   ensures   pure (r == Kuiper.Seq.Common.seq_fold_left d.pure_op zero v_a)
@@ -28,4 +30,6 @@ type reduce_ty
 inline_for_extraction noextract
 val reduce
   (#et : Type0) {| scalar et |} {| has_atomic_add et |}
-  : reduce_ty et
+  (#r : (l:nat -> layout l))
+  {| cr : (l:sz -> Kuiper.Tensor.ctlayout (r l)) |}
+  : reduce_ty et r
