src/lib/inst/Kuiper.AtomicReduce.fsti
@@ -2,9 +2,10 @@ module Kuiper.AtomicReduce
 
 #lang-pulse
 open Kuiper
+open Kuiper.Tensor.Layout.Alg { l1_forward }
 module P = Kuiper.Poly.AtomicReduce
 
-val reduce_u32 : P.reduce_ty u32
-val reduce_u64 : P.reduce_ty u64
-val reduce_f32 : P.reduce_ty f32
-val reduce_f64 : P.reduce_ty f64
+val reduce_u32 : P.reduce_ty u32 l1_forward
+val reduce_u64 : P.reduce_ty u64 l1_forward
+val reduce_f32 : P.reduce_ty f32 l1_forward
+val reduce_f64 : P.reduce_ty f64 l1_forward
